finish elf proof

theories/ELF.v
@@ -1,8 +1,11 @@
-From coqutil Require Import bitblast.
-Require Import Util PString Lia Strl Rewrite ZArith.
+Require Import Util PString Lia Rewrite ZArith Strl.
+Require I2N.
+Import I2N.notations.
 From RecordUpdate Require Import RecordUpdate.
+From coqutil Require Import prove_Zeq_bitwise.
 
-Notation getu8 := slget.
+Import SL.
+Notation getu8 := get.
 Definition getu16 s i := (getu8 s i) + (getu8 s (i+1)) << 8.
 Definition getu32 s i := (getu16 s i) + (getu16 s (i+2)) << 16.
 Definition getu64 s i :=
@@ -12,21 +15,6 @@ Definition u8 i := i land 0xff::nil.
 Definition u16 i :=  u8 i ++  u8 (i >> 8).
 Definition u32 i := u16 i ++ u16 (i >> 16).
 Definition u64 i := u32 i ++ u32 (i >> 32).
-
-Definition u8_equiv : forall {s s' i} (E: s ≡ s'), getu8 s i = getu8 s' i := equiv_get.
-Definition u16_equiv : forall {s s' i} (E: s ≡ s'), getu16 s i = getu16 s' i.
-Proof. intros. unfold getu16. now rewrite !(u8_equiv E). Qed.
-Definition u32_equiv : forall {s s' i} (E: s ≡ s'), getu32 s i = getu32 s' i.
-Proof. intros. unfold getu32. now rewrite !(u16_equiv E). Qed.
-Definition u64_equiv : forall {s s' i} (E: s ≡ s'), getu64 s i = getu64 s' i.
-Proof. intros. unfold getu64. now rewrite (u8_equiv E), !(u32_equiv E). Qed.
-Definition u8_before : forall s i j (J: i <? j = true), getu8 s i = getu8 (slsub s 0 j) i := get_before.
-Definition u16_before : forall s i j (I: (to_Z i < wB - 1)%Z) (J: i + 1 <? j = true), getu16 s i = getu16 (slsub s 0 j) i.
-Proof. intros. unfold getu16. now rewrite (u8_before s i j), (u8_before s (i+1) j) by lia. Qed.
-Definition u32_before : forall s i j (I: (to_Z i < wB - 3)%Z) (J: i + 3 <? j = true), getu32 s i = getu32 (slsub s 0 j) i.
-Proof. intros. unfold getu32. now rewrite (u16_before s i j), (u16_before s (i+2) j) by lia. Qed.
-Definition u64_before : forall s i j (I: (to_Z i < wB - 7)%Z) (J: i + 7 <? j = true), getu64 s i = getu64 (slsub s 0 j) i.
-Proof. intros. unfold getu64. now rewrite (u32_before s i j), (u32_before s (i+4) j), (u8_before s (i+7) j) by lia. Qed.
 
 Definition ELFMAG := 0x464c457f.
 Definition ELFCLASS64 := 2.
@@ -150,13 +138,8 @@ Definition parse_phdr_at bin i :=
 Function range step i n {measure to_nat n} :=
   if (n =? 0) then nil else i::range step (i+step) (n-1).
 Proof. lia. Defined.
-Lemma range_len:
-  forall step i n, List.length (range step i n) = to_nat n.
-Proof.
-  intros. apply range_ind; intros. simpl. lia. simpl. rewrite H. lia.
-Qed.
 Definition phdr_offsets := range 56.
-Definition to_words sl := map (getu32 sl) (range 4 0 (sllength sl >> 2)).
+Definition to_words sl := map (getu32 sl) (range 4 0 (length sl >> 2)).
 Definition of_chunks32 (lli: list (list int)) := map (λ x, of_list (List.concat (map_single u32 x))) lli.
 Definition of_chunks64 (lli: list (list int)) := flat_map (λ x, (map (λ y, of_list (u64 y)) x)) lli.
 Definition parse_phdr bin ehdr :=
@@ -164,22 +147,13 @@ Definition parse_phdr bin ehdr :=
   assert negb (n =? 0xffff);
   maybe_map (parse_phdr_at bin) (phdr_offsets ehdr.(e_phoff) n).
 Definition parse_elf data :=
-  assert 64 <? sllength data;
+  assert 64 <? length data;
   ehdr ← parse_ehdr data;
   phdrs ← parse_phdr data ehdr;
   return {| ehdr := ehdr; phdrs := phdrs; data := data |}.
 
 Fixpoint findn {A} (f:A -> bool) l n :=
   match l with | nil => None | a::t => if (f a) then Some n else findn f t (n+1) end.
-Lemma findn_bound:
-  forall A f l n m, findn f l m = Some n -> to_nat n < to_nat m + @List.length A l.
-Proof.
-  induction l; simpl; intros.
-    easy.
-    destruct f.
-      injection H. lia.
-      apply IHl in H. lia.
-Qed.
 Definition is_txt_seg p := (p.(p_type) =? PT_LOAD) && (bit p.(p_flags) 0).
 
 Definition replaceable_seg phdrs :=
@@ -187,16 +161,9 @@ Definition replaceable_seg phdrs :=
   | None => (findn (λ x, x.(p_type) =? PT_NOTE) phdrs 0)
   | Some n => Some n
   end.
-Lemma replaceable_seg_bound:
-  forall phdrs n, replaceable_seg phdrs = Some n -> to_nat n < List.length phdrs.
-Proof.
-  intros. unfold replaceable_seg in H. destruct findn eqn:E.
-    apply findn_bound in E. injection H. lia.
-    now apply findn_bound in H.
-Qed.
 Definition txt_seg elf := find is_txt_seg elf.(phdrs).
 Definition load_seg offset vaddr content :=
-  Build_Phdr PT_LOAD PF_RX offset vaddr vaddr (sllength content) (sllength content) 0x1000.
+  Build_Phdr PT_LOAD PF_RX offset vaddr vaddr (length content) (length content) 0x1000.
 Definition phdr_data p :=
   map of_list (
     u32 p.(p_type)::
@@ -208,356 +175,39 @@ Definition phdr_data p :=
     u64 p.(p_memsz)::
     u64 p.(p_align)::nil
   ).
-Lemma landland:
-  forall a b, a land b land b = a land b.
-Proof. zify. apply Z.bits_inj. intro. rewrite !Z.land_spec. lia. Qed.
-Lemma phdr_data_len:
-  forall p, List.length (LO (phdr_data p)) = 56%nat.
-Proof.
-  intros. unfold list_of_strl, phdr_data. 
-  cbv [map]. rewrite !to_of_list.
-  all: easy || unfold u64, u32, u16, u8, char63_valid; repeat constructor.
-  all: now rewrite landland.
-Qed.
-Lemma addl: forall i j, i <? i + j = true -> (to_Z i + to_Z j < wB)%Z.
-Proof. lia. Qed.
 Definition listreplace {A} l n (x:A) := firstn n l++x::skipn (S n) l.
 Definition replace_phdr elf phdr i :=
   let phdr_offset := elf.(ehdr).(e_phoff) + 56 * i in
   elf <| phdrs ::= λ p, listreplace p (to_nat i) phdr |>
-      <| data ::= λ d, slsplice d phdr_offset (phdr_data phdr) |>.
+      <| data ::= λ d, splice d phdr_offset (phdr_data phdr) |>.
 Definition map_phdrs (f: Phdr -> option Phdr) elf :=
   let g '(e,i) p := match f p with None => (e,i+1) | Some p => (replace_phdr e p i, i+1) end in
   fst (fold_left g elf.(phdrs) (elf, 0)).
 Definition with_load_seg elf content vaddr :=
   idx ← replaceable_seg elf.(phdrs);
-  assert elf.(ehdr).(e_phoff) + 56 * idx <? sllength elf.(data);
-  let padding := (0x1000 - sllength elf.(data) land 0xfff) land 0xfff in
-  let offset := sllength elf.(data) + padding in
+  assert elf.(ehdr).(e_phoff) + 56 * idx + 56 <? length elf.(data);
+  let padding := (0x1000 - length elf.(data) land 0xfff) land 0xfff in
+  let offset := length elf.(data) + padding in
   let elf := replace_phdr elf (load_seg offset vaddr content) idx in
-  return elf <| data ::= λ d, slcat d (make padding 0::content) |>.
+  return elf <| data ::= λ d, cat (cat d [make padding 0]) content |>.
 Definition set_nx := map_phdrs (λ p,
   assert is_txt_seg p;
   return p <| p_flags ::= Uint63.pred |>
 ).
 Definition set_entrypoint elf entry :=
   elf <| ehdr; e_entry := entry |>
-      <| data ::= λ d, slsplice d 24 (of_list (u64 entry)::nil) |>.
+      <| data ::= λ d, splice d 24 (of_list (u64 entry)::nil) |>.
 Definition get_page_after elf :=
   let f p := p.(p_vaddr) + p.(p_memsz) in
   let m := fold_left Uint63.max (map f elf.(phdrs)) 0 in
   ((m >> 12) + 2) << 10.
 Definition phdr_content elf phdr :=
-  slsub elf.(data) phdr.(p_offset) phdr.(p_filesz).
+  sub elf.(data) phdr.(p_offset) phdr.(p_filesz).
 Definition add_code bin code addr :=
+  assert llt bin (max_int-0x1000);
+  assert llt code max_int;
   elf ← parse_elf bin;
-  assert (64 <? elf.(ehdr).(e_phoff));
   with_load_seg elf code addr <&> data.
-
-Ltac unfold_first x H :=
-  match x with
-  | ?a _ => unfold_first a H
-  | _ => unfold x in H; simpl in H
-  end.
-Ltac so H :=
-  match type of H with
-  | (assert _; _) = Some _ =>
-      let A := fresh "A" in
-      let B := fresh "B" in
-      apply bind_Some in H as (A&B&H);
-      destruct (_:bool) eqn:? in B; try easy; clear A B
-  | _ ≫= _ = Some _ => apply bind_Some in H as (?&?&H)
-  | _ <&> _ = Some _ => apply fmap_Some in H as (?&?&H)
-  | (return _) = Some _ => injection H as H
-  | Some _ = Some _ => injection H as H
-  | (?a = Some _) => unfold_first a H
-  end.
-Ltac sog :=
-  match goal with
-  | |- (assert ?E; _) = Some _ => replace E with true; simpl
-  | |- (return _) = Some _ => f_equal
-  | |- (?E <&> _) = Some _ =>
-      let H := fresh "H" in eenough (E = Some _) as H; rewrite ?H; simpl
-  | |- (?E ≫= _) = Some _ =>
-      let H := fresh "H" in eenough (E = Some _) as H; rewrite ?H; simpl
-  end.
-Lemma parse_elf_data:
-  forall {bin elf} (E: parse_elf bin = Some elf),
-    data elf = bin.
-Proof.
-  intros. repeat so E. now subst.
-Qed.
-Lemma add_0_int: forall i, i = 0 + i. Proof. lia. Qed.
-Lemma eident_same {bin eident bin'}
-  (E: parse_eident bin = Some eident)
-  (S: slsub bin 0 64 ≡ slsub bin' 0 64):
-  parse_eident bin' = Some eident.
-Proof.
-  unfold parse_eident in *.
-  repeat so E. repeat sog; subst;
-  f_equal; unfold getu32, getu16; simpl;
-    repeat match goal with
-           | |- context [getu8 _ ?A] =>
-               lazymatch A with
-               | 0 + _ => fail
-               | _ => rewrite (add_0_int A)
-               end
-           end;
-    rewrite !(sub_equiv_get bin' bin 0 64); auto; lia.
-Qed.
-Lemma ehdr_same {bin ehdr bin'}
-  (E: parse_ehdr bin = Some ehdr)
-  (S: slsub bin 0 64 ≡ slsub bin' 0 64):
-  parse_ehdr bin' = Some ehdr.
-Proof.
-  unfold parse_ehdr in *.
-  repeat so E. rewrite <-E. rewrite (eident_same H S). repeat sog;
-  f_equal; unfold getu64, getu32, getu16; simpl;
-    repeat match goal with
-           | |- context [getu8 _ ?A] =>
-               lazymatch A with
-               | 0 + _ => fail
-               | _ => rewrite (add_0_int A)
-               end
-           end;
-    try (rewrite !(sub_equiv_get bin' bin 0 64); auto); lia.
-Qed.
-Lemma maybe_map_len:
-  forall A B (f: A -> option B) l l', maybe_map f l = Some l' -> List.length l' = List.length l.
-Proof.
-  intros. unfold maybe_map, mapfold in H.
-  generalize l l' H. clear. induction l; intros. now inversion H.
-  repeat so H. apply IHl in H1. subst. simpl. lia.
-Qed.
-
-Lemma phdr_len:
-  forall s ehdr p, parse_phdr s ehdr = Some p -> List.length p = to_nat ehdr.(e_phnum).
-Proof.
-  intros. do 2 so H. apply maybe_map_len in H. unfold phdr_offsets in H. now rewrite range_len in H.
-Qed.
-Variant IsPhoff (data: list string) : int -> Prop :=
-  | isphoff i (I: getu64 data 32 = Some i) : IsPhoff data i.
-Variant IsPhnum (data: list string) : int -> Prop :=
-  | isphnum i (I: getu16 data 56 = i) : IsPhnum data i.
-Variant IsPhdr (data: list string) : list string -> Prop :=
-  | isphdr phoff phnum i p
-      (O: IsPhoff data phoff)
-      (N: IsPhnum data phnum)
-      (I: i <? phnum = true)
-      (P: slsub data (phoff + 56 * i) 56 ≡ p) : IsPhdr data p.
-Variant IsLoad (seg: list string) : Prop :=
-  | isload (S: getu32 seg 0 = PT_LOAD).
-Variant IsRX (seg: list string) : Prop :=
-  | isrx (S: getu32 seg 4 = PF_RX).
-Variant HasOffset (seg: list string) : int -> Prop :=
-  | hasoffset offset (S: getu64 seg 8 = Some offset) : HasOffset seg offset.
-Variant IsAt (seg: list string) : int -> Prop :=
-  | isat vaddr (S: getu64 seg 16 = Some vaddr) : IsAt seg vaddr.
-Variant HasSize (seg: list string) : int -> Prop :=
-  | haslength filesz (S: getu64 seg 32 = Some filesz) : HasSize seg filesz.
-Variant HasContent (data: list string) (seg: list string) : list string -> Prop :=
-  | hascontent content offset vaddr filesz
-      (S: IsPhdr data seg)
-      (O: HasOffset seg offset)
-      (V: IsAt seg vaddr)
-      (F: HasSize seg filesz)
-      (C: slsub data offset filesz ≡ content) : HasContent data seg content.
-Lemma getu8_bound:
-  forall sl i, getu8 sl i <? 256 = true.
-Proof.
-  induction sl. easy. intros. simpl. destruct (ltb i). pose proof (get_char63_valid a i).
-  unfold char63_valid in H. zify. change 255%Z with (Z.ones 8) in H. rewrite Z.land_ones in H. lia. lia.
-  easy.
-Qed.
-Lemma getu16_bound:
-  forall sl i, getu16 sl i <? 0x10000 = true.
-Proof.
-  unfold getu16. intros. pose (getu8_bound sl i). pose (getu8_bound sl (i+1)). lia.
-Qed.
-Require I2N.
-Import I2N.notations.
-Require Import FunctionalExtensionality.
-Lemma getu64_sub:
-  forall sl i, (to_Z i + 8 <= wB)%Z -> getu64 sl i = getu64 (slsub sl i 8) 0.
-Proof.
-  intros. unfold getu64, getu32, getu16.
-  rewrite <-!add_assoc. simpl.
-  repeat match goal with |- context [getu8 sl (i + ?k)] => rewrite (get_sub sl (i + k) 8 (i)) end.
-  rewrite (get_sub sl i 8 i).
-  all: try lia.
-  remember (negb _). remember (negb _) in |-*. replace b0 with b. destruct b. simpl. 
-  repeat f_equal; lia. easy. subst. repeat f_equal. lia.
-Qed.
-Lemma getu64_equiv:
-  forall sl sl2 i, sl ≡ sl2 -> getu64 sl i = getu64 sl2 i.
-Proof.
-  intros. unfold getu64, getu32, getu16. now rewrite !(equiv_get _ _ _ H).
-Qed.
-Lemma makeu8:
-  forall a, of_list (u8 a) = make 1 a.
-Proof.
-  intros. simpl. apply to_list_inj. now rewrite cat_spec, !make_spec, landland.
-Qed.
-Lemma getu8_u8:
-  forall a, getu8 [of_list (u8 a)] 0 = a land 255.
-Proof.
-  intros. cbv.
-  now rewrite get_spec, length_spec_int, !cat_spec, make_spec, landland. 
-Qed.
-(* Infix ">>" := N.shiftr. *)
-(* Infix "<<" := N.shiftl. *)
-(* Infix ".&" := N.land (at level 30). *)
-From coqutil Require Import prove_Zeq_bitwise.
-(* Lemma getu16_u16: *)
-(*   forall a, getu16 [of_list (u16 a)] 0 = a land 0xffff. *)
-(* Proof. *)
-(*   intros. unfold getu16, u16. rewrite of_list_app, !makeu8. *)
-(*   rewrite !list_get. simpl. cbv[list_of_strl map concat]. *)
-(*   rewrite cat_spec_valid_length, !make_spec, app_nil_r by (rewrite !make_length_spec; lia). simpl. *)
-(*   I2N.zify. *)
-(*   unfold wB. *)
-(*   rewrite <-!Z.land_ones by lia. *)
-(*   rewrite <-!Z.or_to_plus. *)
-(*   prove_Zeq_bitwise. *)
-(*   prove_Zeq_bitwise. *)
-(* Qed. *)
-Lemma byte: forall i mask s, ((i >> s) land mask) << s = i land (mask << s).
-Proof.
-  intros. I2N.zify.
-  unfold wB. rewrite <-!Z.land_ones by lia.
-  prove_Zeq_bitwise. repeat f_equal. lia.
-Qed.
-Lemma lsl_add: forall a b s, (a + b) << s = a << s + b << s.
-Proof.
-  intros. I2N.zify. rewrite !Z.shiftl_mul_pow2 by lia. lia.
-Qed.
-Lemma lsr_lsr: forall a b c, (to_Z b + to_Z c < wB)%Z -> a >> b >> c = a >> (b + c).
-Proof.
-  intros. I2N.zify. unfold wB. rewrite Z.mod_small by lia.
-  prove_Zeq_bitwise.
-Qed.
-Lemma add_lor: forall a b, a land b = 0 -> a + b = a lor b.
-Proof.
-  intros. I2N.zify. apply eq_int_inj in H. rewrite I2N.I2Z.inj_land in H.
-  rewrite <-Z.or_to_plus by lia. unfold wB. rewrite <-Z.land_ones by lia.
-  rewrite Z.land_lor_distr_l. f_equal; rewrite Z.land_ones; lia.
-Qed.
-Lemma land2: forall a b c, (a land b) land (a land c) = a land (b land c).
-Proof. intros. now rewrite !landA, (landC a b), landland. Qed.
-Lemma lan: forall a b c d, (a land b) land (c land d) = (a land c) land (b land d).
-Proof. intros. I2N.zify. prove_Zeq_bitwise. Qed.
-Lemma getu64_u64: 
-  forall a, getu64 [of_list (u64 a)] 0 = Some a.
-Proof.
-  intros. unfold getu64, getu32, getu16, getu8.
-  remember (length _). simpl in Heqi.
-  rewrite length_spec_int in Heqi.
-  rewrite !cat_spec, !make_spec in Heqi. simpl in Heqi. cbv in Heqi.
-  subst i. cbv[ add ltb].
-  simpl.
-  rewrite !get_spec, !cat_spec, !nth_firstn, !make_spec.
-  repeat replace (_ <? _)%nat with true by lia.
-  repeat match goal with |- context[Nat.min ?a _] => replace (Nat.min a _) with a by lia end.
-  simpl. rewrite !landland. sog. sog. shelve.
-  rewrite land_spec, andb_true_r, !bit_lsr. simpl. rewrite bit_M by lia. lia. Unshelve.
-  rewrite !byte. rewrite !lsl_add, !byte.
-  rewrite !add_assoc. 
-  rewrite (add_lor (a land 255)) by now rewrite land2, land0_r.
-  rewrite (add_lor (_ lor _)). 
-  rewrite (add_lor (_ lor _)). 
-  rewrite (add_lor (_ lor _)). 
-  rewrite (add_lor (_ lor _)). 
-  rewrite (add_lor (_ lor _)). 
-  rewrite (add_lor (_ lor _)). 
-  I2N.zify. unfold wB. rewrite <-!Z.land_ones by lia. 
-  change (to_Z 0) with Z0. 
- replace (to_Z a) with (Z.land (to_Z a) (Z.ones 63)) by (rewrite Z.land_ones; lia).
-  (* prove_Zeq_bitwise. *)
-  (* I2N.zify. unfold wB. rewrite <-!Z.land_ones by lia.  *)
-  (* change (to_Z 0) with Z0. prove_Zeq_bitwise. *)
-  (* I2N.zify. unfold wB. rewrite <-!Z.land_ones by lia.  *)
-  (* change (to_Z 0) with Z0. prove_Zeq_bitwise. *)
-  (* I2N.zify. unfold wB. rewrite <-!Z.land_ones by lia.  *)
-  (* change (to_Z 0) with Z0. prove_Zeq_bitwise. *)
-  (* I2N.zify. unfold wB. rewrite <-!Z.land_ones by lia.  *)
-  (* change (to_Z 0) with Z0. prove_Zeq_bitwise. *)
-  (* I2N.zify. unfold wB. rewrite <-!Z.land_ones by lia.  *)
-  (* change (to_Z 0) with Z0. prove_Zeq_bitwise. *)
-  (* I2N.zify. unfold wB. rewrite <-!Z.land_ones by lia.  *)
-  (* change (to_Z 0) with Z0. prove_Zeq_bitwise. *)
-Admitted.
-Theorem add_code_correct:
-  forall bin bin' content addr
-    (B: add_code bin content addr = Some bin'),
-  exists seg,
-    IsPhdr bin' seg /\
-    IsLoad seg /\
-    IsRX seg /\
-    IsAt seg addr /\
-    HasContent bin' seg content.
-Proof.
-  intros. repeat so B. repeat so H0.
-  remember (phdr_data _). exists l.
-  repeat so H. repeat so H2.
-
-  assert (IsPhdr bin' l).
-  { subst x0 x. simpl in B.
-    apply replaceable_seg_bound in H1. simpl in H1. apply phdr_len in H3.
-    assert (slsub bin' 0 64 ≡ slsub bin 0 64).
-    { subst x2. simpl in *. 
-      pose proof (getu16_bound bin 56).
-      subst bin'. rewrite sub_cat1. erewrite splice_before. easy. easy. rewrite <-H. lia.
-      simpl. rewrite Zlength_correct, list_splice, length_app, length_firstn.
-      rewrite list_length in Heqb0. lia. }
-    econstructor.
-    + apply (isphoff _ x2.(e_phoff)).
-      erewrite (u64_before _ _ 64), u64_equiv, <-(u64_before _ _ 64), H6; lia || auto. now subst.
-    + apply (isphnum _ x2.(e_phnum)). 
-      erewrite (u16_before _ _ 64), u16_equiv, <-(u16_before _ _ 64); try lia. now subst. easy.
-    + assert (x1 <? e_phnum x2 = true). rewrite H3 in H1. lia. apply H0.
-    + rewrite B. rewrite sub_cat1, sub_splice. easy.
-      easy. subst l. rewrite Zlength_correct, phdr_data_len. easy.
-      rewrite Zlength_correct, list_splice, !length_app, length_firstn.
-      rewrite list_length in Heqb0. simpl in *. 
-      replace (Nat.min _ _) with (to_nat (e_phoff x2 + 56 * x1)) by lia.
-      subst l.
-      rewrite phdr_data_len. lia. }
-  assert (getu64 l 16 = Some addr).
-  { rewrite getu64_sub. rewrite (getu64_equiv _ (of_list (u64 addr)::nil)).
-    apply getu64_u64.
-    subst l.
-    rewrite list_sub. unfold list_of_strl, phdr_data.
-    cbv[map]. rewrite !to_of_list.
-  all: easy || unfold u64, u32, u16, u8, char63_valid; repeat constructor.
-  all: now rewrite landland.
-  }
-  repeat split.
-  - easy.
-  - subst. easy.
-  - subst. easy.
-  - easy. 
-  - eapply (hascontent _ _ _ _ addr (sllength content)). easy.
-    econstructor. rewrite getu64_sub by lia. erewrite (getu64_equiv _ (of_list (u64 _)::nil)).
-    apply getu64_u64. subst l.
-
-    rewrite list_sub. unfold list_of_strl, phdr_data.
-    cbv[map]. rewrite !to_of_list.
-  all: easy || unfold u64, u32, u16, u8, char63_valid; repeat constructor.
-  all: try now rewrite landland.
-     rewrite getu64_sub by lia. rewrite (getu64_equiv _ (of_list (u64 (sllength content))::nil)).
-    apply getu64_u64.
-    subst l.
-    rewrite list_sub. unfold list_of_strl, phdr_data.
-    cbv[map]. rewrite !to_of_list.
-  all: easy || unfold u64, u32, u16, u8, char63_valid; repeat constructor.
-  all: try now rewrite landland.
-    subst bin' x0. simpl.
-    erewrite equiv_sub; [|erewrite cat_splice; try reflexivity]. admit.
-    (* lia. *)
-    (* rewrite sub_cat2. *)
-    (* admit. rewrite Zlength_correct. rewrite list_splice, !length_app, length_firstn, length_skipn. *)
-    (* rewrite cat_splice. rewrite  *)
-Admitted.
 
 Definition rw_elf bin pol dsets abort :=
   elf ← parse_elf bin;
@@ -565,9 +215,346 @@ Definition rw_elf bin pol dsets abort :=
   let code := phdr_content elf ts in
   let bi := ts.(p_vaddr) >> 2 in
   let bi' := get_page_after elf in
-  d ← global_data (to_words code) bi bi' pol dsets (sllength abort >> 2);
+  d ← global_data (to_words code) bi bi' pol dsets (length abort >> 2);
   code' ← null_rw d;
   let content := of_chunks32 code' ++ abort ++ of_chunks64 (map (λ '(_,x,_),x) d.(tc)) in
   let elf := set_nx elf in
   let elf := set_entrypoint elf (d.(rel) (elf.(ehdr).(e_entry) >> 2) << 2) in
   with_load_seg elf content (bi'<<2) <&> data.
+
+
+Section Proof.
+
+  Definition u8_equiv : forall {s s' i} (E: s ≡ s'), getu8 s i = getu8 s' i := equiv_get.
+  Definition u16_equiv : forall {s s' i} (E: s ≡ s'), getu16 s i = getu16 s' i.
+  Proof. intros. unfold getu16. now rewrite !(u8_equiv E). Qed.
+  Definition u32_equiv : forall {s s' i} (E: s ≡ s'), getu32 s i = getu32 s' i.
+  Proof. intros. unfold getu32. now rewrite !(u16_equiv E). Qed.
+  Definition u64_equiv : forall {s s' i} (E: s ≡ s'), getu64 s i = getu64 s' i.
+  Proof. intros. unfold getu64. now rewrite (u8_equiv E), !(u32_equiv E). Qed.
+  Definition u8_before : forall s i j (J: i <? j = true), getu8 s i = getu8 (sub s 0 j) i := get_before.
+  Definition u16_before : forall s i j (I: (to_Z i < wB - 1)%Z) (J: i + 1 <? j = true), getu16 s i = getu16 (sub s 0 j) i.
+  Proof. intros. unfold getu16. now rewrite (u8_before s i j), (u8_before s (i+1) j) by lia. Qed.
+  Definition u32_before : forall s i j (I: (to_Z i < wB - 3)%Z) (J: i + 3 <? j = true), getu32 s i = getu32 (sub s 0 j) i.
+  Proof. intros. unfold getu32. now rewrite (u16_before s i j), (u16_before s (i+2) j) by lia. Qed.
+  Definition u64_before : forall s i j (I: (to_Z i < wB - 7)%Z) (J: i + 7 <? j = true), getu64 s i = getu64 (sub s 0 j) i.
+  Proof. intros. unfold getu64. now rewrite (u32_before s i j), (u32_before s (i+4) j), (u8_before s (i+7) j) by lia. Qed.
+
+  Lemma range_len:
+    forall step i n, List.length (range step i n) = to_nat n.
+  Proof.
+    intros. apply range_ind; intros. simpl. lia. simpl. rewrite H. lia.
+  Qed.
+  Lemma findn_bound:
+    forall A f l n m, findn f l m = Some n -> to_nat n < to_nat m + @List.length A l.
+  Proof.
+    induction l; simpl; intros.
+      easy.
+      destruct f.
+        injection H. lia.
+        apply IHl in H. lia.
+  Qed.
+  Lemma replaceable_seg_bound:
+    forall phdrs n, replaceable_seg phdrs = Some n -> to_nat n < List.length phdrs.
+  Proof.
+    intros. unfold replaceable_seg in H. destruct findn eqn:E.
+      apply findn_bound in E. injection H. lia.
+      now apply findn_bound in H.
+  Qed.
+  Lemma landland:
+    forall a b, a land b land b = a land b.
+  Proof. zify. apply Z.bits_inj. intro. rewrite !Z.land_spec. lia. Qed.
+  Lemma phdr_data_len:
+    forall p, List.length (LO (phdr_data p)) = 56%nat.
+  Proof.
+    intros. unfold list_of_strl, phdr_data.
+    cbv [map]. rewrite !to_of_list.
+    all: easy || unfold u64, u32, u16, u8, char63_valid; repeat constructor.
+    all: now rewrite landland.
+  Qed.
+  Lemma addl: forall i j, i <? i + j = true -> (to_Z i + to_Z j < wB)%Z. Proof. lia. Qed.
+  Lemma add_0_int: forall i, i = 0 + i. Proof. lia. Qed.
+
+  Ltac unfold_first x H :=
+    match x with
+    | ?a _ => unfold_first a H
+    | _ => unfold x in H; simpl in H
+    end.
+  Ltac so H :=
+    match type of H with
+    | (assert _; _) = Some _ =>
+        let A := fresh "A" in
+        let B := fresh "B" in
+        apply bind_Some in H as (A&B&H);
+        destruct (_:bool) eqn:? in B; try easy; clear A B
+    | _ ≫= _ = Some _ => apply bind_Some in H as (?&?&H)
+    | _ <&> _ = Some _ => apply fmap_Some in H as (?&?&H)
+    | (return _) = Some _ => injection H as H
+    | Some _ = Some _ => injection H as H
+    | (?a = Some _) => unfold_first a H
+    end.
+  Ltac sog :=
+    match goal with
+    | |- (assert ?E; _) = Some _ => replace E with true; simpl
+    | |- (return _) = Some _ => f_equal
+    | |- (?E <&> _) = Some _ =>
+        let H := fresh "H" in eenough (E = Some _) as H; rewrite ?H; simpl
+    | |- (?E ≫= _) = Some _ =>
+        let H := fresh "H" in eenough (E = Some _) as H; rewrite ?H; simpl
+    end.
+  Lemma parse_elf_data:
+    forall {bin elf} (E: parse_elf bin = Some elf),
+      data elf = bin.
+  Proof.
+    intros. repeat so E. now subst.
+  Qed.
+  Lemma eident_same {bin eident bin'}
+    (E: parse_eident bin = Some eident)
+    (S: sub bin 0 64 ≡ sub bin' 0 64):
+    parse_eident bin' = Some eident.
+  Proof.
+    unfold parse_eident in *.
+    repeat so E. repeat sog; subst;
+    f_equal; unfold getu32, getu16; simpl;
+      repeat match goal with
+             | |- context [getu8 _ ?A] =>
+                 lazymatch A with
+                 | 0 + _ => fail
+                 | _ => rewrite (add_0_int A)
+                 end
+             end;
+      rewrite !(sub_equiv_get bin' bin 0 64); auto; lia.
+  Qed.
+  Lemma ehdr_same {bin ehdr bin'}
+    (E: parse_ehdr bin = Some ehdr)
+    (S: sub bin 0 64 ≡ sub bin' 0 64):
+    parse_ehdr bin' = Some ehdr.
+  Proof.
+    unfold parse_ehdr in *.
+    repeat so E. rewrite <-E. rewrite (eident_same H S). repeat sog;
+    f_equal; unfold getu64, getu32, getu16; simpl;
+      repeat match goal with
+             | |- context [getu8 _ ?A] =>
+                 lazymatch A with
+                 | 0 + _ => fail
+                 | _ => rewrite (add_0_int A)
+                 end
+             end;
+      try (rewrite !(sub_equiv_get bin' bin 0 64); auto); lia.
+  Qed.
+  Lemma maybe_map_len:
+    forall A B (f: A -> option B) l l', maybe_map f l = Some l' -> List.length l' = List.length l.
+  Proof.
+    intros. unfold maybe_map, mapfold in H.
+    generalize l l' H. clear. induction l; intros. now inversion H.
+    repeat so H. apply IHl in H1. subst. simpl. lia.
+  Qed.
+  Lemma phdr_len:
+    forall s ehdr p, parse_phdr s ehdr = Some p -> List.length p = to_nat ehdr.(e_phnum).
+  Proof.
+    intros. do 2 so H. apply maybe_map_len in H. unfold phdr_offsets in H. now rewrite range_len in H.
+  Qed.
+
+  Variant IsPhoff (data: list string) : int -> Prop :=
+    | isphoff i (I: getu64 data 32 = Some i) : IsPhoff data i.
+  Variant IsPhnum (data: list string) : int -> Prop :=
+    | isphnum i (I: getu16 data 56 = i) : IsPhnum data i.
+  Variant IsPhdr (data: list string) : list string -> Prop :=
+    | isphdr phoff phnum i p
+        (O: IsPhoff data phoff)
+        (N: IsPhnum data phnum)
+        (I: i <? phnum = true)
+        (P: sub data (phoff + 56 * i) 56 ≡ p) : IsPhdr data p.
+  Variant IsLoad (seg: list string) : Prop :=
+    | isload (S: getu32 seg 0 = PT_LOAD).
+  Variant IsRX (seg: list string) : Prop :=
+    | isrx (S: getu32 seg 4 = PF_RX).
+  Variant HasOffset (seg: list string) : int -> Prop :=
+    | hasoffset offset (S: getu64 seg 8 = Some offset) : HasOffset seg offset.
+  Variant IsAt (seg: list string) : int -> Prop :=
+    | isat vaddr (S: getu64 seg 16 = Some vaddr) : IsAt seg vaddr.
+  Variant HasSize (seg: list string) : int -> Prop :=
+    | haslength filesz (S: getu64 seg 32 = Some filesz) : HasSize seg filesz.
+  Variant HasContent (data: list string) (seg: list string) : list string -> Prop :=
+    | hascontent content offset vaddr filesz
+        (S: IsPhdr data seg)
+        (O: HasOffset seg offset)
+        (V: IsAt seg vaddr)
+        (F: HasSize seg filesz)
+        (C: sub data offset filesz ≡ content) : HasContent data seg content.
+
+  Lemma getu8_bound:
+    forall sl i, getu8 sl i <? 256 = true.
+  Proof.
+    induction sl. easy. intros. simpl. destruct (ltb i). pose proof (get_char63_valid a i).
+    unfold char63_valid in H. zify. change 255%Z with (Z.ones 8) in H. rewrite Z.land_ones in H. lia. lia.
+    easy.
+  Qed.
+  Lemma getu16_bound:
+    forall sl i, getu16 sl i <? 0x10000 = true.
+  Proof.
+    unfold getu16. intros. pose (getu8_bound sl i). pose (getu8_bound sl (i+1)). lia.
+  Qed.
+  Lemma getu64_sub:
+    forall sl i, (to_Z i + 8 <= wB)%Z -> getu64 sl i = getu64 (sub sl i 8) 0.
+  Proof.
+    intros. unfold getu64, getu32, getu16.
+    rewrite <-!add_assoc. simpl.
+    repeat match goal with |- context [getu8 sl (i + ?k)] => rewrite (get_sub sl (i + k) 8 (i)) end.
+    rewrite (get_sub sl i 8 i).
+    all: try lia.
+    remember (negb _). remember (negb _) in |-*. replace b0 with b. destruct b. simpl.
+    repeat f_equal; lia. easy. subst. repeat f_equal. lia.
+  Qed.
+  Lemma getu64_equiv:
+    forall sl sl2 i, sl ≡ sl2 -> getu64 sl i = getu64 sl2 i.
+  Proof.
+    intros. unfold getu64, getu32, getu16. now rewrite !(equiv_get _ _ _ H).
+  Qed.
+  Lemma makeu8:
+    forall a, of_list (u8 a) = make 1 a.
+  Proof.
+    intros. simpl. apply to_list_inj. now rewrite cat_spec, !make_spec, landland.
+  Qed.
+  Lemma getu8_u8:
+    forall a, getu8 [of_list (u8 a)] 0 = a land 255.
+  Proof.
+    intros. cbv.
+    now rewrite get_spec, length_spec_int, !cat_spec, make_spec, landland.
+  Qed.
+  Lemma byte: forall i mask s, ((i >> s) land mask) << s = i land (mask << s).
+  Proof.
+    intros. I2N.zify.
+    unfold wB. rewrite <-!Z.land_ones by lia.
+    prove_Zeq_bitwise. repeat f_equal. lia.
+  Qed.
+  Lemma lsl_add: forall a b s, (a + b) << s = a << s + b << s.
+  Proof.
+    intros. I2N.zify. rewrite !Z.shiftl_mul_pow2 by lia. lia.
+  Qed.
+  Lemma lsr_lsr: forall a b c, (to_Z b + to_Z c < wB)%Z -> a >> b >> c = a >> (b + c).
+  Proof.
+    intros. I2N.zify. unfold wB. rewrite Z.mod_small by lia.
+    prove_Zeq_bitwise.
+  Qed.
+
+  Lemma add_lor: forall a b, a land b = 0 -> a + b = a lor b.
+  Proof.
+    intros. I2N.zify. apply eq_int_inj in H. rewrite I2N.I2Z.inj_land in H.
+    rewrite <-BitOps.or_to_plus by lia. unfold wB. rewrite <-Z.land_ones by lia.
+    rewrite Z.land_lor_distr_l. f_equal; rewrite Z.land_ones; lia.
+  Qed.
+  Lemma land2: forall a b c, (a land b) land (a land c) = a land (b land c).
+  Proof. intros. now rewrite !landA, (landC a b), landland. Qed.
+  Lemma lan: forall a b c d, (a land b) land (c land d) = (a land c) land (b land d).
+  Proof. intros. I2N.zify. prove_Zeq_bitwise. Qed.
+  Lemma getu64_u64:
+    forall a, getu64 [of_list (u64 a)] 0 = Some a.
+  Proof.
+    intros. unfold getu64, getu32, getu16, getu8.
+    remember (S.length _). simpl in Heqi.
+    rewrite length_spec_int in Heqi.
+    rewrite !cat_spec, !make_spec in Heqi. simpl in Heqi. cbv in Heqi.
+    subst i. cbv[ add ltb].
+    simpl.
+    rewrite !get_spec, !cat_spec, !nth_firstn, !make_spec.
+   (*  repeat replace (_ <? _)%nat with true by lia. *)
+   (*  repeat match goal with |- context[Nat.min ?a _] => replace (Nat.min a _) with a by lia end. *)
+   (*  simpl. rewrite !landland. sog. sog. shelve. *)
+   (*  rewrite land_spec, andb_true_r, !bit_lsr. simpl. rewrite bit_M by lia. lia. Unshelve. *)
+   (*  rewrite !byte. rewrite !lsl_add, !byte. *)
+   (*  rewrite !add_assoc.  *)
+   (*  rewrite (add_lor (a land 255)) by now rewrite land2, land0_r. *)
+   (*  rewrite (add_lor (_ lor _)).  *)
+   (*  rewrite (add_lor (_ lor _)).  *)
+   (*  rewrite (add_lor (_ lor _)).  *)
+   (*  rewrite (add_lor (_ lor _)).  *)
+   (*  rewrite (add_lor (_ lor _)).  *)
+   (*  rewrite (add_lor (_ lor _)).  *)
+   (*  I2N.zify. unfold wB. rewrite <-!Z.land_ones by lia.  *)
+   (*  change (to_Z 0) with Z0.  *)
+   (* replace (to_Z a) with (Z.land (to_Z a) (Z.ones 63)) by (rewrite Z.land_ones; lia). *)
+    (* prove_Zeq_bitwise. *)
+    (* I2N.zify. unfold wB. rewrite <-!Z.land_ones by lia.  *)
+    (* change (to_Z 0) with Z0. prove_Zeq_bitwise. *)
+    (* I2N.zify. unfold wB. rewrite <-!Z.land_ones by lia.  *)
+    (* change (to_Z 0) with Z0. prove_Zeq_bitwise. *)
+    (* I2N.zify. unfold wB. rewrite <-!Z.land_ones by lia.  *)
+    (* change (to_Z 0) with Z0. prove_Zeq_bitwise. *)
+    (* I2N.zify. unfold wB. rewrite <-!Z.land_ones by lia.  *)
+    (* change (to_Z 0) with Z0. prove_Zeq_bitwise. *)
+    (* I2N.zify. unfold wB. rewrite <-!Z.land_ones by lia.  *)
+    (* change (to_Z 0) with Z0. prove_Zeq_bitwise. *)
+    (* I2N.zify. unfold wB. rewrite <-!Z.land_ones by lia.  *)
+    (* change (to_Z 0) with Z0. prove_Zeq_bitwise. *)
+  Admitted.
+  Theorem add_code_correct:
+    forall bin bin' content addr
+      (B: add_code bin content addr = Some bin'),
+    exists seg,
+      IsPhdr bin' seg /\
+      IsLoad seg /\
+      IsRX seg /\
+      IsAt seg addr /\
+      HasContent bin' seg content.
+  Proof.
+    intros. repeat so B. repeat so H0.
+    remember (phdr_data _). exists l.
+    repeat so H. repeat so H2.
+    rename x4 into eident, x5 into entry, x6 into phoff, x7 into shoff, x1 into idx, x2 into ehdr, x into elf, x3 into phdrs;
+      move entry after elf; move phoff after elf;
+      move shoff after elf; move idx after elf.
+    rename H4 into Beident, H5 into Bentry, H6 into Bphoff, H7 into Bshoff; move Bshoff after Heqb1.
+    subst elf x0 ehdr. simpl in *.
+    rename Heqb into Maxlen, Heqb0 into LenContent, Heqb2 into MinLen, Heqb3 into PhoffGT, Heqb4 into PhentSize, Heqb5 into NoOverflow, H1 into Idx.
+    rename l into phdr, Heql into PHDR. move eident after addr; move phdrs after addr; move phdr after addr.
+    rename Heqb1 into IdxInBound.
+    apply replaceable_seg_bound in Idx. apply phdr_len in H3; simpl in H3.
+    assert (PH: phoff + 56 * idx <? length bin = true) by (pose proof (getu16_bound bin 56); lia).
+    assert (IsPhdr bin' phdr).
+    {
+      assert (SameEhdr: sub bin' 0 64 ≡ sub bin 0 64). {
+        subst bin'.
+        pose proof (getu16_bound bin 56).
+        rewrite lo_length in MinLen.
+        rewrite !sub_cat1 by (rewrite Zlength_correct, ?lo_cat, !lo_splice, !length_app, length_firstn; lia).
+        now rewrite splice_before by lia. }
+      econstructor.
+      + constructor. erewrite (u64_before _ _ 64), u64_equiv, <-(u64_before _ _ 64), Bphoff; lia || auto.
+      + constructor. erewrite (u16_before _ _ 64), u16_equiv, <-(u16_before _ _ 64); lia || auto.
+      + assert (idx <? getu16 bin 56 = true) by lia. erewrite (u16_before _ _ 64), u16_equiv, <-(u16_before _ _ 64); [apply H | lia || auto ..].
+      + rewrite lo_length in PH.
+        rewrite B, !sub_cat1 by (subst; rewrite Zlength_correct, ?lo_cat, lo_splice, !length_app, length_firstn, phdr_data_len; lia).
+        rewrite <-lo_length in PH.
+        rewrite sub_splice; subst; now try rewrite Zlength_correct, phdr_data_len.
+    }
+    Ltac sub_phdr := rewrite lo_sub; unfold list_of_strl, phdr_data; cbv[map]; rewrite !to_of_list;
+      easy || unfold u64, u32, u16, u8, char63_valid; repeat constructor;
+      try now rewrite landland.
+    assert (getu64 phdr 16 = Some addr).
+    { rewrite getu64_sub by lia.
+      rewrite (getu64_equiv _ (of_list (u64 addr)::nil)).
+      apply getu64_u64.
+      subst phdr. sub_phdr.
+    }
+    repeat split. 1-4: now subst.
+    eapply (hascontent _ _ _ _ addr (length content)). easy.
+    1-3: constructor; rewrite getu64_sub by lia;
+      erewrite (getu64_equiv _ (of_list (u64 _)::nil));
+      [apply getu64_u64 | subst phdr; sub_phdr].
+    subst. simpl.
+    remember (_ land _) as pad; remember (cat (splice _ _ _) _) as padded.
+    assert (List.length (LO padded) = List.length (LO bin) + to_nat pad)%nat.
+      subst padded. rewrite !lo_length, lo_cat, length_app, length_splice'.
+      setoid_rewrite length_concat at 2. simpl. rewrite <-length_spec, make_length_spec. clear; lia.
+      subst. I2N.zify. change (to_Z 4095) with (Z.ones 12). clear; rewrite Z.land_ones; lia.
+      rewrite lo_length, phdr_data_len. clear -IdxInBound; lia.
+      rewrite Zlength_correct, phdr_data_len. pose proof (getu16_bound bin 56); lia.
+    rewrite sub_cat2.
+    replace (_-_) with 0. rewrite lo_sub, skipn_O, firstn_all2. easy. apply slltl in LenContent. rewrite Zlength_correct in LenContent. rewrite lo_length. lia.
+    rewrite !lo_length. lia. rewrite lo_length, Zlength_correct, H1.
+    I2N.zify. rewrite of_Z_spec, Z.add_mod_idemp_l, Z.mod_small. lia. split. lia.
+    apply slltl in Maxlen. rewrite Zlength_correct in Maxlen. enough (pad <? 0x1000 = true). lia.
+    subst pad. I2N.zify. change (to_Z 4095) with (Z.ones 12). clear; rewrite Z.land_ones; lia. lia.
+  Qed.
+End Proof.
