theories/Strl.v
@@ -2,53 +2,57 @@ Require Import List Uint63 PString Recdef Lia ZifyUint63 ZArith Utf8.
 Open Scope uint63.
 Open Scope pstring.
 
-Fixpoint slget sl i :=
-  match sl with
-  | nil => 0
-  | a::t =>
-      if (i <? length a)
-      then get a i
-      else slget t (i - length a)
-  end.
-Definition slcat := @app string.
-Fixpoint slsub sl i n :=
-  if (n =? 0) then nil else
-  match sl with
-  | nil => nil
-  | a::t =>
-      if (i <? length a) then
-        let x := sub a i n in
-        x::slsub t 0 (n - length x)
-      else
-        slsub t (i - length a) n
-  end.
-Definition sllength sl := List.fold_left add (map length sl) 0.
-Fixpoint sldrop sl n :=
-  if (n =? 0) then sl else
-  match sl with
-  | nil => nil
-  | a::t =>
-      if (n <? length a) then
-        sub a n (length a)::t
-      else
-        sldrop t (n - length a)
-  end.
-Fixpoint sllt sl n :=
-  if (n =? 0) then false else
-  match sl with
-  | nil => true
-  | a::t =>
-      if (n <? length a) then false
-      else sllt t (n - length a)
-  end.
-Definition slsplice sl i sl2 :=
-  slcat (slcat (slsub sl 0 i) sl2) (sldrop sl (i + sllength sl2)).
+Module S := PrimString.
+Module SL.
+  Fixpoint get sl i :=
+    match sl with
+    | nil => 0
+    | a::t =>
+        if (i <? length a)
+        then PrimString.get a i
+        else get t (i - length a)
+    end.
+  Definition cat := @app string.
+  Fixpoint sub sl i n :=
+    if (n =? 0) then nil else
+    match sl with
+    | nil => nil
+    | a::t =>
+        if (i <? length a) then
+          let x := PrimString.sub a i n in
+          x::sub t 0 (n - length x)
+        else
+          sub t (i - length a) n
+    end.
+  Definition length sl := List.fold_left add (map length sl) 0.
+  Fixpoint drop sl n :=
+    if (n =? 0) then sl else
+    match sl with
+    | nil => nil
+    | a::t =>
+        if (n <? PrimString.length a) then
+          PrimString.sub a n (PrimString.length a)::t
+        else
+          drop t (n - PrimString.length a)
+    end.
+  Fixpoint llt sl n :=
+    if (n =? 0) then false else
+    match sl with
+    | nil => true
+    | a::t =>
+        if (n <? PrimString.length a) then false
+        else llt t (n - PrimString.length a)
+    end.
+  Definition splice sl i sl2 :=
+    cat (cat (sub sl 0 i) sl2) (drop sl (i + length sl2)).
+End SL.
+Import SL.
 Definition list_of_strl sl := List.concat (map to_list sl).
 Notation "'LO'" := list_of_strl.
-Notation slequiv sl1 sl2 := (list_of_strl sl1 = list_of_strl sl2).
-Infix "≡" := slequiv.
-Lemma list_get:
-  forall sl i, slget sl i = nth (to_nat i) (LO sl) 0.
+Notation equiv sl1 sl2 := (list_of_strl sl1 = list_of_strl sl2).
+Infix "≡" := equiv.
+Lemma lo_get:
+  forall sl i, get sl i = nth (to_nat i) (LO sl) 0.
 Proof.
   induction sl; intros; unfold list_of_strl.
     simpl. now destruct (_:nat).
@@ -58,13 +62,13 @@ Proof.
     rewrite IHsl. rewrite app_nth2, <-length_spec. f_equal. lia.
     rewrite <-length_spec. lia.
 Qed.
-Lemma list_cat:
-  forall sl1 sl2, LO (slcat sl1 sl2) = LO sl1 ++ LO sl2.
+Lemma lo_cat:
+  forall sl1 sl2, LO (cat sl1 sl2) = LO sl1 ++ LO sl2.
 Proof.
-  intros. unfold slcat, list_of_strl. now rewrite map_app, concat_app.
+  intros. unfold cat, list_of_strl. now rewrite map_app, concat_app.
 Qed.
-Lemma list_sub:
-  forall sl i n, LO (slsub sl i n) = firstn (to_nat n) (skipn (to_nat i) (LO sl)).
+Lemma lo_sub:
+  forall sl i n, LO (sub sl i n) = firstn (to_nat n) (skipn (to_nat i) (LO sl)).
 Proof.
   unfold list_of_strl. induction sl; intros; simpl.
     destruct eqb; now rewrite skipn_nil, firstn_nil.
@@ -80,8 +84,8 @@ Proof.
         f_equal. rewrite <-length_spec. lia.
         rewrite <-length_spec. lia.
 Qed.
-Lemma list_drop:
-  forall sl n, LO (sldrop sl n) = skipn (to_nat n) (LO sl).
+Lemma lo_drop:
+  forall sl n, LO (drop sl n) = skipn (to_nat n) (LO sl).
 Proof.
   unfold list_of_strl. induction sl; intros; simpl.
     destruct eqb; now rewrite skipn_nil.
@@ -100,35 +104,35 @@ Lemma fold_add:
 Proof.
   induction l. simpl. lia. simpl. intro. rewrite IHl, (IHl (0+a)). lia.
 Qed.
-Lemma list_length:
-  forall sl, sllength sl = of_nat (List.length (LO sl)).
+Lemma lo_length:
+  forall sl, length sl = of_nat (List.length (LO sl)).
 Proof.
   intros. unfold list_of_strl.
   induction sl. easy.
-  unfold sllength in *. simpl. rewrite fold_add.
+  unfold length in *. simpl. rewrite fold_add.
   rewrite IHsl. rewrite length_app. rewrite <-length_spec. lia.
 Qed.
-Lemma list_splice:
+Lemma lo_splice:
   forall sl1 i sl2,
-    LO (slsplice sl1 i sl2) =
-    firstn (to_nat i) (LO sl1)++LO sl2++skipn (to_nat (i + sllength sl2)) (LO sl1).
+    LO (splice sl1 i sl2) =
+    firstn (to_nat i) (LO sl1)++LO sl2++skipn (to_nat (i + length sl2)) (LO sl1).
 Proof.
-  intros. unfold slsplice.
-  rewrite !list_cat, !list_sub, list_drop, skipn_O, app_assoc. f_equal.
+  intros. unfold splice.
+  now rewrite !lo_cat, !lo_sub, lo_drop, skipn_O, app_assoc.
 Qed.
 
 Lemma equiv_get:
-  forall sl1 sl2 i, sl1 ≡ sl2 -> slget sl1 i = slget sl2 i.
+  forall sl1 sl2 i, sl1 ≡ sl2 -> get sl1 i = get sl2 i.
 Proof.
-  intros. now rewrite !list_get, H.
+  intros. now rewrite !lo_get, H.
 Qed.
 Lemma sub_equiv_get:
-  forall sl1 sl2 i j, slsub sl1 i j ≡ slsub sl2 i j ->
+  forall sl1 sl2 i j, sub sl1 i j ≡ sub sl2 i j ->
   (to_Z i + to_Z j < wB)%Z ->
   forall k, k <? j = true ->
-  slget sl1 (i+k) = slget sl2 (i+k).
+  get sl1 (i+k) = get sl2 (i+k).
 Proof.
-  intros. rewrite !list_get. rewrite !list_sub in H.
+  intros. rewrite !lo_get. rewrite !lo_sub in H.
   replace (to_nat _) with (to_nat i + to_nat k)%nat by lia.
   rewrite <-!nth_skipn.
   apply (f_equal (λ l, nth (to_nat k) l 0)) in H.
@@ -136,76 +140,76 @@ Proof.
   now replace _ with true in H by lia.
 Qed.
 Definition get_before:
-  forall sl i j, i <? j = true -> slget sl i = slget (slsub sl 0 j) i.
+  forall sl i j, i <? j = true -> get sl i = get (sub sl 0 j) i.
 Proof.
   intros. replace i with (0 + i). erewrite sub_equiv_get. easy.
-  now rewrite !list_sub, !skipn_O, firstn_firstn, Nat.min_id.
+  now rewrite !lo_sub, !skipn_O, firstn_firstn, Nat.min_id.
   all: lia.
 Qed.
 Definition get_sub:
-  forall sl i j k, k <=? i = true -> i - k <? j = true -> slget sl i = slget (slsub sl k j) (i - k).
+  forall sl i j k, k <=? i = true -> i - k <? j = true -> get sl i = get (sub sl k j) (i - k).
 Proof.
-  intros. rewrite !list_get, list_sub.
+  intros. rewrite !lo_get, lo_sub.
   rewrite nth_firstn. replace (_ <? _)%nat with true by lia.
   rewrite nth_skipn. f_equal. lia.
 Qed.
 Lemma splice_before:
-  forall sl1 sl2 i j, i <? sllength sl1 = true -> i <? j = true ->
-  slsub (slsplice sl1 j sl2) 0 i ≡ slsub sl1 0 i.
+  forall sl1 sl2 i j, i <=? length sl1 = true -> i <=? j = true ->
+  sub (splice sl1 j sl2) 0 i ≡ sub sl1 0 i.
 Proof.
-  intros. unfold slsplice.
-  rewrite !list_sub, !list_cat, !list_sub, !skipn_O, <-app_assoc.
+  intros. unfold splice.
+  rewrite !lo_sub, !lo_cat, !lo_sub, !skipn_O, <-app_assoc.
   rewrite firstn_app, length_firstn, firstn_firstn.
-  replace (_ - _)%nat with O by (rewrite list_length in H; lia).
+  replace (_ - _)%nat with O by (rewrite lo_length in H; lia).
   rewrite firstn_O, app_nil_r. f_equal. lia.
 Qed.
 Lemma sub_splice:
   forall sl1 sl2 i j,
-    i <? sllength sl1 = true -> 
+    i <? length sl1 = true ->
     to_Z j = Zlength (LO sl2) ->
-    slsub (slsplice sl1 i sl2) i j ≡ sl2.
+    sub (splice sl1 i sl2) i j ≡ sl2.
 Proof.
-  intros. rewrite list_sub, list_splice.
+  intros. rewrite lo_sub, lo_splice.
   rewrite skipn_app, length_firstn, skipn_firstn_comm, Nat.sub_diag, firstn_O, app_nil_l.
-  rewrite list_length in H. replace (_-_)%nat with O by lia.
+  rewrite lo_length in H. replace (_-_)%nat with O by lia.
   rewrite skipn_O, firstn_app. rewrite Zlength_correct in H0.
   replace (_-_)%nat with O by lia. rewrite firstn_O, app_nil_r, firstn_all2.
   easy. lia.
 Qed.
 
 Lemma equiv_sub:
-  forall sl1 sl2 i j, sl1 ≡ sl2 -> slsub sl1 i j ≡ slsub sl2 i j.
+  forall sl1 sl2 i j, sl1 ≡ sl2 -> sub sl1 i j ≡ sub sl2 i j.
 Proof.
-  intros. now rewrite !list_sub, H.
+  intros. now rewrite !lo_sub, H.
 Qed.
 Lemma cat_splice:
-  forall sl1 sl2 sl3 i, i + sllength sl2 <? sllength sl1 = true ->
+  forall sl1 sl2 sl3 i, i + length sl2 <? length sl1 = true ->
   (to_Z i + Zlength (LO sl2) < wB)%Z ->
-  slcat (slsplice sl1 i sl2) sl3 ≡ slsplice (slcat sl1 sl3) i sl2.
+  cat (splice sl1 i sl2) sl3 ≡ splice (cat sl1 sl3) i sl2.
 Proof.
-  intros. rewrite list_cat, !list_splice, list_cat, <-!app_assoc.
+  intros. rewrite lo_cat, !lo_splice, lo_cat, <-!app_assoc.
   rewrite Zlength_correct in H0.
-  f_equal. rewrite firstn_app. rewrite !list_length in H. replace (_ - _)%nat with O. now rewrite app_nil_r. lia.
+  f_equal. rewrite firstn_app. rewrite !lo_length in H. replace (_ - _)%nat with O. now rewrite app_nil_r. lia.
   rewrite skipn_app. replace (_ - _)%nat with O. easy.
-  rewrite !list_length in *. lia.
+  rewrite !lo_length in *. lia.
 Qed.
 Lemma sub_cat:
-  forall sl1 sl2 i j, i+j <? sllength sl1 = true ->
+  forall sl1 sl2 i j, i+j <? length sl1 = true ->
   (to_Z i + to_Z j < wB)%Z ->
-  slsub (slcat sl1 sl2) i j ≡ slsub sl1 i j.
+  sub (cat sl1 sl2) i j ≡ sub sl1 i j.
 Proof.
-  intros. rewrite !list_sub, list_cat.
+  intros. rewrite !lo_sub, lo_cat.
   rewrite skipn_app, firstn_app.
   replace (_ - _)%nat with O.
   now rewrite firstn_O, app_nil_r.
-  rewrite length_skipn. rewrite list_length in H. lia.
+  rewrite length_skipn. rewrite lo_length in H. lia.
 Qed.
 Lemma sub_cat1:
   forall sl1 sl2 i j,
   (to_Z i + to_Z j <= Zlength (LO sl1))%Z ->
-  slsub (slcat sl1 sl2) i j ≡ slsub sl1 i j.
+  sub (cat sl1 sl2) i j ≡ sub sl1 i j.
 Proof.
-  intros. rewrite !list_sub, list_cat.
+  intros. rewrite !lo_sub, lo_cat.
   rewrite skipn_app, firstn_app.
   replace (_ - _)%nat with O.
   now rewrite firstn_O, app_nil_r.
@@ -214,15 +218,15 @@ Qed.
 Lemma sub_cat2:
   forall sl1 sl2 i j,
   (Zlength (LO sl1) <= to_Z i)%Z ->
-  slsub (slcat sl1 sl2) i j ≡ slsub sl2 (i - sllength sl1) j.
+  sub (cat sl1 sl2) i j ≡ sub sl2 (i - length sl1) j.
 Proof.
-  intros. rewrite !list_sub, list_cat.
+  intros. rewrite !lo_sub, lo_cat.
   rewrite Zlength_correct in H.
   rewrite skipn_app, skipn_all2, app_nil_l by lia.
-  repeat f_equal. rewrite list_length. lia.
+  repeat f_equal. rewrite lo_length. lia.
 Qed.
 Lemma slltl:
-  forall sl n, sllt sl n = true <-> (Zlength (LO sl) < to_Z n)%Z.
+  forall sl n, llt sl n = true <-> (Zlength (LO sl) < to_Z n)%Z.
 Proof.
   setoid_rewrite Zlength_correct.
   induction sl; intros; simpl.
@@ -236,20 +240,20 @@ Proof.
           apply IHsl. lia.
 Qed.
 Lemma length_splice:
-  forall sl1 i sl2, i + sllength sl2 <? sllength sl1 = true ->
+  forall sl1 i sl2, i + length sl2 <? length sl1 = true ->
   (to_Z i + Zlength (LO sl2) < wB)%Z ->
-  sllength (slsplice sl1 i sl2) = sllength sl1.
+  length (splice sl1 i sl2) = length sl1.
 Proof.
-  intros. rewrite Zlength_correct, !list_length in *.
-  rewrite list_splice, !length_app, length_firstn, length_skipn, !list_length in *. lia.
+  intros. rewrite Zlength_correct, !lo_length in *.
+  rewrite lo_splice, !length_app, length_firstn, length_skipn, !lo_length in *. lia.
 Qed.
 Lemma length_splice':
-  forall sl1 i sl2, i + sllength sl2 <? sllength sl1 = true ->
+  forall sl1 i sl2, i + length sl2 <? length sl1 = true ->
   (to_Z i + Zlength (LO sl2) < wB)%Z ->
-  List.length (LO (slsplice sl1 i sl2)) = List.length (LO sl1).
+  List.length (LO (splice sl1 i sl2)) = List.length (LO sl1).
 Proof.
-  intros. rewrite Zlength_correct, !list_length in *.
-  rewrite list_splice, !length_app, length_firstn, length_skipn, !list_length in *. lia.
+  intros. rewrite Zlength_correct, !lo_length in *.
+  rewrite lo_splice, !length_app, length_firstn, length_skipn, !lo_length in *. lia.
 Qed.
 Lemma equiv_trans:
   forall sl1 sl2 sl3, sl1 ≡ sl2 -> sl2 ≡ sl3 -> sl1 ≡ sl3.
